src/FiatToFacade/GLabelMapFacts.v
@@ -1,0 +1,7 @@
+
+  Require Import GLabelMap.
+  Require Import FMapFacts.
+  Include (Properties GLabelMap).
+  Include (Facts GLabelMap).
+  Require Import FMapFacts1.
+  Include (WFacts_fun GLabelKey.GLabel_as_OT GLabelMap).
